theories/iSL/SequentProps.v
@@ -18,9 +18,15 @@ Logic (65):4.
 
 (** ** Weakening *)
 
+Lemma open_boxes_add'
+     {K : Kind} (Γ : @env K) (φ : @form K) : (⊗ (Γ • φ)) = (⊗ Γ • ⊙ φ).
+Proof. apply open_boxes_add. Qed.
+(*
+Global Hint Rewrite open_boxes_add' : proof.
+*)
 (** We prove the admissibility of the weakening rule. *)
 
-Theorem weakening φ' Γ φ : Γ ⊢ φ -> Γ•φ' ⊢ φ.
+Theorem weakening {K : Kind} φ' Γ φ : Γ ⊢ φ -> Γ•φ' ⊢ φ.
 Proof with (auto with proof).
 intro H. revert φ'.  induction H; intro φ'; auto with proof; try (exch 0; auto with proof).
 - constructor 4. exch 1; exch 0...
@@ -33,12 +39,12 @@ intro H. revert φ'.  induction H; intro φ'; auto with proof; try (exch 0; auto
 - apply ImpBox; box_tac.
   + peapply (IHProvable1 (open_box φ')).
   + exch 0...
-- apply BoxR. box_tac; exch 0...
+- apply BoxR. box_tac. exch 0...
 Qed.
 
 Global Hint Resolve weakening : proof.
 
-Theorem generalised_weakeningL (Γ Γ' : env) φ: Γ ⊢ φ -> Γ' ⊎ Γ ⊢ φ.
+Theorem generalised_weakeningL {K : Kind} (Γ Γ' : env) φ: Γ ⊢ φ -> Γ' ⊎ Γ ⊢ φ.
 Proof.
 intro Hp.
 induction Γ' as [| x Γ' IHΓ'] using gmultiset_rec.
@@ -46,7 +52,7 @@ induction Γ' as [| x Γ' IHΓ'] using gmultiset_rec.
 - peapply (weakening x). exact IHΓ'. ms.
 Qed.
 
-Theorem generalised_weakeningR (Γ Γ' : env) φ: Γ' ⊢ φ -> Γ' ⊎ Γ ⊢ φ.
+Theorem generalised_weakeningR {K : Kind} (Γ Γ' : env) φ: Γ' ⊢ φ -> Γ' ⊎ Γ ⊢ φ.
 Proof.
 intro Hp.
 induction Γ as [| x Γ IHΓ] using gmultiset_rec.
@@ -62,7 +68,7 @@ Global Hint Extern 5 (?a <= ?b) => simpl in *; lia : proof.
   left, or left, top left (i.e., the appliction of weakening for the formula
   top), the four implication left rules, the and right rule and the application of the or right rule with bottom. *)
 
-Lemma ImpR_rev Γ φ ψ :
+Lemma ImpR_rev {K : Kind} Γ φ ψ :
   (Γ ⊢ (φ →  ψ))
     -> Γ•φ ⊢  ψ.
 Proof with (auto with proof).
@@ -74,13 +80,13 @@ intro Hp. dependent induction Hp; auto with proof; try exch 0.
 - constructor 11. exch 1; exch 0...
 - constructor 12; exch 0...
 - constructor 13; box_tac...
-  + exch 1; exch 0...
+  + exch 1; exch 0. apply weakening...
   + exch 0. auto with proof.
 Qed.
 
 Global Hint Resolve ImpR_rev : proof.
 
-Theorem generalised_axiom Γ φ : Γ•φ ⊢ φ.
+Theorem generalised_axiom {K : Kind} Γ φ : Γ • φ ⊢ φ.
 Proof with (auto with proof).
 remember (weight φ) as w.
 assert(Hle : weight φ ≤ w) by lia.
@@ -88,7 +94,7 @@ clear Heqw. revert Γ φ Hle.
 induction w; intros Γ φ Hle.
 - assert (Hφ := weight_pos φ). lia.
 - destruct φ; simpl in Hle...
-  destruct φ1 as [v| | θ1 θ2 | θ1 θ2 | θ1 θ2 | θ].
+  dependent destruction φ1.
   + constructor 8. exch 0...
   + auto with proof.
   + apply ImpR, AndL. exch 1; exch 0. apply ImpLAnd.
@@ -105,7 +111,7 @@ Global Hint Resolve generalised_axiom : proof.
 Local Ltac lazy_apply th:=
 (erewrite proper_Provable;  [| |reflexivity]);  [eapply th|].
 
-Lemma open_box_L Γ φ ψ : Γ • φ ⊢ ψ -> Γ • ⊙ φ ⊢ ψ.
+Lemma open_box_L {K : Kind} Γ φ ψ : Γ • φ ⊢ ψ -> Γ • ⊙ φ ⊢ ψ.
 Proof.
 intro Hp.
 remember (Γ•φ) as Γ' eqn:HH.
@@ -122,7 +128,8 @@ dependent induction Hp generalizing Γ' Hp; intros φ0 Hin.
 - apply AndR; auto.
 - case (decide (φ0 = (φ ∧ ψ))).
   + intro; subst. simpl. apply AndL. peapply Hp.
-  + intro. forward. apply AndL. do 2 backward. peapply (IHHp φ0). ms.
+  + intro. forward. apply AndL. exch 0. do 2 backward.
+    peapply (IHHp); trivial. ms.
 - apply OrR1; auto.
 - apply OrR2; auto.
 - case (decide (φ0 = (φ ∨ ψ))).
@@ -130,71 +137,71 @@ dependent induction Hp generalizing Γ' Hp; intros φ0 Hin.
       * peapply Hp1.
       * peapply Hp2.
   + intro. forward. apply OrL.
-      * backward. peapply (IHHp1 φ0). ms.
-      * backward. peapply (IHHp2 φ0). ms.
-- apply ImpR. backward. apply IHHp. ms.
+      * backward. peapply IHHp1; trivial. ms.
+      * backward. peapply IHHp2; trivial. ms.
+- apply ImpR. backward. apply IHHp; trivial. ms.
 - case (decide (φ0 = Var p)).
   + intro; subst; simpl. forward. apply ImpLVar. peapply Hp.
   + intro. case (decide (φ0 = (Var p → φ))).
-      * intro; subst; simpl. peapply ImpLVar. exact Hp. ms.
+      * intro; subst; simpl. peapply (ImpLVar Γ). exact Hp. ms.
       * intro. do 2 forward. exch 0. apply ImpLVar. exch 0. do 2 backward.
-         apply IHHp. ms.
+         apply IHHp; trivial. ms.
 - case (decide (φ0 =  (φ1 ∧ φ2 → φ3))).
   + intro; subst; simpl. apply ImpLAnd. peapply Hp. 
-  + intro. forward. apply ImpLAnd. backward. apply IHHp. ms.
+  + intro. forward. apply ImpLAnd. backward. apply IHHp; trivial. ms.
 - case (decide (φ0 =  (φ1 ∨ φ2 → φ3))).
   + intro; subst; simpl. apply ImpLOr. peapply Hp.
-  + intro. forward. apply ImpLOr. exch  0. do 2 backward. apply IHHp. ms.
+  + intro. forward. apply ImpLOr. exch  0. do 2 backward. apply IHHp; trivial. ms.
 - case (decide (φ0 =  ((φ1 → φ2) → φ3))).
   + intro; subst; simpl. apply ImpLImp. peapply Hp1. peapply Hp2.
   + intro. forward. apply ImpLImp.
-      * backward. apply IHHp1. ms.
-      * backward. apply IHHp2. ms.
+      * backward. apply IHHp1; trivial. ms.
+      * backward. apply IHHp2; trivial. ms.
 - case (decide (φ0 =  (□ φ1 → φ2))).
   + intro; subst; simpl. apply ImpBox.
-      * lazy_apply Hp1; autorewrite with proof; ms.
+      * box_tac. lazy_apply Hp1. autorewrite with proof. ms.
       * peapply Hp2.
   + intro. forward.
       case (decide (open_box φ0 = □ φ1)).
       * intro Heq. repeat rewrite Heq. apply ImpBox; box_tac.
         -- exch 1; exch 0. apply generalised_axiom.
-        -- backward. rewrite <- Heq. apply IHHp2. auto with *.
+        -- backward. rewrite <- Heq. apply IHHp2; trivial. auto with *.
       * intro Hneq. case (decide (open_box φ0 = φ2)).
           -- intro Heq. subst φ2. apply ImpBox; box_tac.
-              ++ (erewrite proper_Provable;  [| |reflexivity]);  [eapply (IHHp1 (⊙ φ0))|].
-                      ms.
-                      autorewrite with proof; [|ms]. repeat rewrite env_replace.
+              ++ (erewrite proper_Provable;  [| |reflexivity]);  [eapply (IHHp1 (⊙ φ0))|]. ms.
+                 autorewrite with proof; [|ms]. repeat rewrite env_replace.
                      ** ms.
                      ** auto with proof.
                      ** apply env_in_add. right. auto with proof; ms.
-              ++ box_tac. backward. apply (IHHp2 φ0). auto with *.
+              ++ box_tac. backward. apply IHHp2; trivial. auto with *.
           -- intro Hneq'. apply ImpBox; repeat box_tac.
             ++ exch 0. box_tac. assert((⊙ φ0) ∈ (⊗ Γ)) by (now apply In_open_boxes).
-                    backward. backward. eapply (IHHp1 (⊙ φ0)). ms.
-            ++ backward. apply IHHp2.  apply env_in_add. now right.
+                    backward. backward. eapply IHHp1; trivial. ms.
+            ++ backward. apply IHHp2; trivial. apply env_in_add. now right.
 - case (decide (open_box φ0 = □ φ)).
   + intro Heq; rewrite Heq. apply generalised_axiom.
   + intro. backward. apply BoxR. box_tac.
       case (decide (open_box φ0 = open_box (open_box φ0))).
       * intro Heq. lazy_apply Hp. autorewrite with proof. rewrite <- Heq. ms. ms.
       * intro. assert( open_box φ0 ∈ open_boxes Γ) by (now apply In_open_boxes).
-         lazy_apply (IHHp (open_box φ0)).
+        lazy_apply (IHHp (open_box φ0)).
         -- ms.
         -- autorewrite with proof. repeat rewrite env_replace; ms. ms.
 Qed.
 
 Local Hint Resolve env_in_add : proof.
 
-Lemma open_boxes_R (Γ : env) (φ ψ : form): (Γ • φ) ⊢ ψ → ((⊗Γ) • φ) ⊢ ψ.
+Lemma open_boxes_R {K : Kind} (Γ : env) φ ψ: (Γ • φ) ⊢ ψ → (⊗Γ) • φ ⊢ ψ.
 Proof.
 revert ψ.
 induction Γ using gmultiset_rec; intro ψ.
 - rewrite open_boxes_empty. trivial.
-- intro HP. lazy_apply (open_box_L  (⊗ Γ • φ) x ψ).
+- intro HP. lazy_apply (open_box_L (⊗ Γ • φ) x ψ).
   + apply ImpR_rev, IHΓ, ImpR. peapply HP.
   + rewrite open_boxes_disj_union, open_boxes_singleton; ms.
 Qed.
-Lemma AndL_rev Γ φ ψ θ: (Γ•φ ∧ ψ) ⊢ θ  → (Γ•φ•ψ) ⊢ θ.
+
+Lemma AndL_rev {K : Kind} Γ φ ψ θ: (Γ•φ ∧ ψ) ⊢ θ  → (Γ•φ•ψ) ⊢ θ.
 Proof.
 intro Hp.
 remember (Γ•φ ∧ ψ) as Γ' eqn:HH.
@@ -203,30 +210,31 @@ assert(Hin : (φ ∧ ψ) ∈ Γ')by ms.
 rw Heq 2. clear Γ HH Heq. revert φ ψ Hin.
 (* we massaged the goal so that the environment of the derivation on which we do
    the induction is not composite anymore *)
-induction Hp; intros φ0 ψ0 Hin; try forward.
+induction Hp; intros φ0 ψ0 Hin.
 (* auto takes care of the right rules easily *)
-- auto with proof.
-- auto with proof.
+- forward. auto with proof.
+- forward. auto with proof.
 - apply AndR; auto with proof.
 (* the main case *)
-- case(decide ((φ ∧ ψ) = (φ0 ∧ ψ0))); intro Heq0.
-  + inversion Heq0; subst. peapply Hp.
+- (* TODO: forward gets stuck there. *)
+  case(decide ((φ ∧ ψ) = (φ0 ∧ ψ0))); intro Heq0.
+  + dependent destruction Heq0; subst. peapply Hp.
   + forward. constructor 4. exch 0. backward. backward. apply IHHp. ms.
 (* only left rules remain. Now it's all a matter of putting the right principal
    formula at the front, apply the rule; and put back the front formula at the back
    before applying the induction hypothesis *)
 - apply OrR1. auto with proof.
 - apply OrR2. auto with proof.
-- constructor 7; backward; [apply IHHp1 | apply IHHp2]; ms.
+- forward. constructor 7; backward; [apply IHHp1 | apply IHHp2]; ms.
 - constructor 8. backward. apply IHHp. ms.
-- forward. exch 0. constructor 9. exch 0. do 2 backward. apply IHHp. ms.
-- constructor 10. backward. apply IHHp. ms.
-- constructor 11. exch 0. do 2 backward. apply IHHp. ms.
-- constructor 12; backward.
+- forward. forward. exch 0. constructor 9. exch 0. do 2 backward. apply IHHp. ms.
+- forward. constructor 10. backward. apply IHHp. ms.
+- forward. constructor 11. exch 0. do 2 backward. apply IHHp. ms.
+- forward. constructor 12; backward.
   + apply IHHp1. ms.
   + apply IHHp2. ms.
-- constructor 13; repeat box_tac.
-  + exch 0.  box_tac.
+- forward. constructor 13; repeat box_tac.
+  + exch 0. box_tac.
       apply In_open_boxes in Hin0. backward. backward. apply open_box_L. exch 0. apply open_box_L. exch 0. 
       apply IHHp1. ms.
   + backward. apply IHHp2. ms.
@@ -239,7 +247,7 @@ induction Hp; intros φ0 ψ0 Hin; try forward.
       apply In_open_boxes in Hin. auto with proof.
 Qed.
 
-Lemma OrL_rev Γ φ ψ θ: (Γ•φ ∨ ψ) ⊢ θ  → (Γ•φ ⊢ θ)  * (Γ•ψ ⊢ θ).
+Lemma OrL_rev {K : Kind} Γ φ ψ θ: (Γ•φ ∨ ψ) ⊢ θ  → (Γ•φ ⊢ θ) * (Γ•ψ ⊢ θ).
 Proof.
 intro Hp.
 remember (Γ•φ ∨ ψ) as Γ' eqn:HH.
@@ -251,12 +259,12 @@ clear Γ HH Heq.
 induction Hp.
 - split; forward; auto with proof.
 - split; forward; auto with proof.
-- split; constructor 3; intuition.
+- split; constructor 3; now (apply IHHp1 || apply IHHp2).
 - split; forward; constructor 4; exch 0; do 2 backward; apply IHHp; ms.
-- split; constructor 5; intuition.
-- split; apply OrR2; intuition.
+- split; constructor 5; now apply IHHp.
+- split; apply OrR2; now apply IHHp.
 - case (decide ((φ0 ∨ ψ0) = (φ ∨ ψ))); intro Heq0.
-  + inversion Heq0; subst. split; [peapply Hp1| peapply Hp2].
+  + dependent destruction Heq0; subst. split; [peapply Hp1| peapply Hp2].
   + split; forward; constructor 7; backward; (apply IHHp1||apply IHHp2); ms.
 - split; constructor 8; backward; apply IHHp; ms.
 - split; do 2 forward; exch 0; constructor 9; exch 0; do 2 backward; apply IHHp; ms.
@@ -264,15 +272,20 @@ induction Hp.
 - split; forward; constructor 11; exch 0; do 2 backward; apply IHHp; ms.
 - split; forward; constructor 12; backward; (apply IHHp1 || apply IHHp2); ms.
 - split; forward; assert(Hin' : (φ ∨ ψ) ∈ (⊗ Γ • □ φ1 • φ2))
-  by (apply env_in_add; right; apply env_in_add; right; auto with proof);
-  assert((φ ∨ ψ) ∈ ⊗Γ) by auto with proof;
+  by (apply env_in_add; right; apply env_in_add; right; eauto with proof);
+  assert((φ ∨ ψ) ∈ ⊗Γ) by eauto with proof;
   (constructor 13; repeat box_tac; exch 0;
     [do 2 backward; apply open_box_L; apply IHHp1|exch 0; backward; apply IHHp2];ms).
--  assert (Hin' : (φ ∨ ψ) ∈ (⊗ Γ • □ φ0)) by (apply env_in_add; right; auto with proof).
+-  assert (Hin' : (φ ∨ ψ) ∈ (⊗ Γ • □ φ0)) by (apply env_in_add; right; eauto with proof).
     split; constructor 14; repeat box_tac; backward; apply open_box_L; now apply IHHp.
 Qed.
+(*
+Lemma open_boxes_spec Γ φ : φ ∈ open_boxes Γ -> {φ ∈ Γ ∧ is_box φ = false} + {(□ φ) ∈ Γ}.
+Admitted.
+  Global Hint Resolve open_boxes_spec : proof.
 
-Lemma TopL_rev Γ φ θ: Γ•(⊥ → φ) ⊢ θ -> Γ ⊢ θ.
+*)
+Lemma TopL_rev {K : Kind} Γ φ θ: Γ•(⊥ → φ) ⊢ θ -> Γ ⊢ θ.
 Proof.
 remember (Γ•(⊥ → φ)) as Γ' eqn:HH.
 assert (Heq: Γ ≡ Γ' ∖ {[ ⊥ → φ ]}) by ms.
@@ -299,58 +312,58 @@ Qed.
 
 Local Hint Immediate TopL_rev : proof.
 
-Lemma ImpLVar_rev Γ p φ ψ: (Γ•Var p•(p → φ)) ⊢ ψ  → (Γ•Var p•φ) ⊢ ψ.
+Lemma ImpLVar_rev {K : Kind} Γ p φ ψ: (Γ•Var p•(p → φ)) ⊢ ψ  → (Γ•Var p•φ) ⊢ ψ.
 Proof.
 intro Hp.
 remember (Γ•Var p•(p → φ)) as Γ' eqn:HH.
 assert (Heq: (Γ•Var p) ≡ Γ' ∖ {[Var p → φ]}) by ms.
 assert(Hin : (p → φ) ∈ Γ')by ms.
 rw Heq 1. clear Γ HH Heq.
-induction Hp; try forward.
-- auto with proof.
-- auto with proof.
+induction Hp.
+- forward; auto with proof.
+- forward; auto with proof.
 - apply AndR; auto with proof.
-- apply AndL. exch 0. do 2 backward. apply IHHp. ms.
+- forward; apply AndL. exch 0. do 2 backward. apply IHHp. ms.
 - apply OrR1. auto with proof.
 - apply OrR2. auto with proof.
-- apply OrL; backward; apply IHHp1 || apply IHHp2; ms.
+- forward; apply OrL; backward; apply IHHp1 || apply IHHp2; ms.
 - apply ImpR. backward. apply IHHp. ms.
 - case (decide ((Var p0 → φ0) = (Var p → φ))); intro Heq0.
-  + inversion Heq0; subst. peapply Hp.
+  + dependent destruction Heq0; subst. peapply Hp.
   + do 2 forward. exch 0. apply ImpLVar. exch 0; do 2 backward. apply IHHp. ms.
-- apply ImpLAnd. backward. apply IHHp. ms.
-- apply ImpLOr. exch 0; do 2 backward. apply IHHp. ms.
-- apply ImpLImp; backward; (apply IHHp1 || apply IHHp2); ms.
--  apply ImpBox; repeat box_tac.
+- forward; apply ImpLAnd. backward. apply IHHp. ms.
+- forward; apply ImpLOr. exch 0; do 2 backward. apply IHHp. ms.
+- forward; apply ImpLImp; backward; (apply IHHp1 || apply IHHp2); ms.
+- forward; apply ImpBox; repeat box_tac.
    +  exch 0; do 2 backward. apply open_box_L. apply IHHp1. ms.
-   + backward.  apply IHHp2. ms.
-- apply BoxR.  repeat box_tac. backward. apply open_box_L. apply IHHp. ms.
+   + backward. apply IHHp2. ms.
+- apply BoxR. repeat box_tac. backward. apply open_box_L. apply IHHp. ms.
 Qed.
 
 (* inversion for ImpLImp is only partial *)
-Lemma ImpLImp_prev Γ φ1 φ2 φ3 ψ: (Γ•((φ1 → φ2) → φ3)) ⊢ ψ -> (Γ•φ3) ⊢ ψ.
+Lemma ImpLImp_prev {K : Kind} Γ φ1 φ2 φ3 ψ: (Γ•((φ1 → φ2) → φ3)) ⊢ ψ -> (Γ•φ3) ⊢ ψ.
 Proof.
 intro Hp.
 remember (Γ •((φ1 → φ2) → φ3)) as Γ' eqn:HH.
 assert (Heq: Γ ≡ Γ' ∖ {[ ((φ1 → φ2) → φ3) ]}) by ms.
 assert(Hin :((φ1 → φ2) → φ3) ∈ Γ')by ms.
 rw Heq 1. clear Γ HH Heq.
-induction Hp; try forward.
-- auto with proof.
-- auto with proof.
+induction Hp.
+- forward; auto with proof.
+- forward; auto with proof.
 - apply AndR; auto with proof.
-- apply AndL. exch 0; do 2 backward. apply IHHp. ms.
+- forward; apply AndL. exch 0; do 2 backward. apply IHHp. ms.
 - apply OrR1. auto with proof.
 - apply OrR2. auto with proof.
--  apply OrL; backward; [apply IHHp1 | apply IHHp2]; ms.
+- forward; apply OrL; backward; [apply IHHp1 | apply IHHp2]; ms.
 - apply ImpR. backward. apply IHHp. ms.
-- forward. exch 0. apply ImpLVar. exch 0. do 2 backward. apply IHHp. ms.
-- apply ImpLAnd. backward. apply IHHp. ms.
-- apply ImpLOr. exch 0. do 2 backward. apply IHHp. ms.
+- do 2 forward. exch 0. apply ImpLVar. exch 0. do 2 backward. apply IHHp. ms.
+- forward; apply ImpLAnd. backward. apply IHHp. ms.
+- forward; apply ImpLOr. exch 0. do 2 backward. apply IHHp. ms.
 - case (decide (((φ0 → φ4) → φ5) = ((φ1 → φ2) → φ3))); intro Heq0.
-  + inversion Heq0; subst. peapply Hp2.
+  + dependent destruction Heq0; subst. peapply Hp2.
   + forward. apply ImpLImp; backward; (apply IHHp1 || apply IHHp2); ms.
--  apply ImpBox; repeat box_tac.
+- forward; apply ImpBox; repeat box_tac.
   + exch 0; do 2 backward. apply open_box_L. apply IHHp1. ms.
   + backward. apply IHHp2. ms.
 - apply BoxR. repeat box_tac. backward. apply open_box_L. apply IHHp. ms.
@@ -364,79 +377,82 @@ remember (Γ •((□φ1) → φ2)) as Γ' eqn:HH.
 assert (Heq: Γ ≡ Γ' ∖ {[ ((□φ1) → φ2) ]}) by ms.
 assert(Hin :((□φ1) → φ2) ∈ Γ')by ms.
 rw Heq 1. clear Γ HH Heq.
-induction Hp; try forward.
-- auto with proof.
-- auto with proof.
+dependent induction Hp.
+- forward; auto with proof.
+- forward; auto with proof.
 - apply AndR; auto with proof.
-- apply AndL. exch 0; do 2 backward. apply IHHp. ms.
+- forward; apply AndL. exch 0; do 2 backward. apply IHHp; trivial. ms.
 - apply OrR1. auto with proof.
 - apply OrR2. auto with proof.
--  apply OrL; backward; [apply IHHp1 | apply IHHp2]; ms.
-- apply ImpR. backward. apply IHHp. ms.
-- forward. exch 0. apply ImpLVar. exch 0. do 2 backward. apply IHHp. ms.
-- apply ImpLAnd. backward. apply IHHp. ms.
-- apply ImpLOr. exch 0. do 2 backward. apply IHHp. ms.
-- apply ImpLImp; backward; (apply IHHp1 || apply IHHp2); ms.
+- forward; apply OrL; backward; [apply IHHp1 | apply IHHp2]; ms.
+- apply ImpR. backward. apply IHHp; trivial. ms.
+- do 2 forward. exch 0. apply ImpLVar. exch 0. do 2 backward.
+  apply IHHp; trivial. ms.
+- forward; apply ImpLAnd. backward. apply IHHp; trivial. ms.
+- forward; apply ImpLOr. exch 0. do 2 backward. apply IHHp; trivial. ms.
+- forward; apply ImpLImp; backward. 
+  + apply IHHp1; trivial. ms.
+  + apply IHHp2; trivial. ms.
 - case (decide((□φ0 → φ3) = (□φ1 → φ2))).
-  + intro Heq; inversion Heq; subst. peapply Hp2.
+  + intro Heq; dependent destruction Heq; subst. peapply Hp2.
   + intro Hneq. forward. apply ImpBox; repeat box_tac.
-     * exch 0; do 2 backward. apply open_box_L; apply IHHp1. ms.
-     * backward. apply IHHp2. ms.
-- apply BoxR. repeat box_tac. backward. apply open_box_L. apply IHHp. ms.
+     * exch 0; do 2 backward. apply open_box_L; apply IHHp1; trivial. ms.
+     * backward. apply IHHp2; trivial. ms.
+- apply BoxR. repeat box_tac. backward. apply open_box_L. apply IHHp; trivial. ms.
 Qed.
 
-
-Lemma ImpLOr_rev Γ φ1 φ2 φ3 ψ: Γ•((φ1 ∨ φ2) → φ3) ⊢ ψ -> Γ•(φ1 → φ3)•(φ2 → φ3) ⊢ ψ.
+Lemma ImpLOr_rev {K : Kind} Γ φ1 φ2 φ3 ψ:
+  Γ•((φ1 ∨ φ2) → φ3) ⊢ ψ -> Γ•(φ1 → φ3)•(φ2 → φ3) ⊢ ψ.
 Proof.
 intro Hp.
 remember (Γ •((φ1 ∨ φ2) → φ3)) as Γ' eqn:HH.
 assert (Heq: Γ ≡ Γ' ∖ {[ ((φ1 ∨ φ2) → φ3) ]}) by ms.
 assert(Hin :((φ1 ∨ φ2) → φ3) ∈ Γ')by ms.
 rw Heq 2. clear Γ HH Heq.
-induction Hp; try forward.
-- auto with proof.
-- auto with proof.
+induction Hp.
+- forward; auto with proof.
+- forward; auto with proof.
 - apply AndR; auto with proof.
-- constructor 4. exch 0; do 2 backward. apply IHHp. ms.
+- forward; constructor 4. exch 0; do 2 backward. apply IHHp. ms.
 - apply OrR1. auto with proof.
 - apply OrR2. auto with proof.
-- constructor 7; backward; [apply IHHp1 | apply IHHp2]; ms.
+- forward; constructor 7; backward; [apply IHHp1 | apply IHHp2]; ms.
 - constructor 8. backward. apply IHHp. ms.
-- forward. exch 0. constructor 9. exch 0. do 2 backward. apply IHHp. ms.
-- constructor 10. backward. apply IHHp. ms.
+- do 2 forward. exch 0. constructor 9. exch 0. do 2 backward. apply IHHp. ms.
+- forward; constructor 10. backward. apply IHHp. ms.
 - case (decide (((φ0 ∨ φ4) → φ5) = ((φ1 ∨ φ2) → φ3))); intro Heq0.
-  + inversion Heq0; subst. peapply Hp.
+  + dependent destruction Heq0; subst. peapply Hp.
   + forward. constructor 11; exch 0; do 2 backward; apply IHHp; ms.
-- constructor 12; backward; (apply IHHp1 || apply IHHp2); ms.
--  apply ImpBox; repeat box_tac.
+- forward; constructor 12; backward; (apply IHHp1 || apply IHHp2); ms.
+- forward; apply ImpBox; repeat box_tac.
   + exch 0; do 2 backward. apply IHHp1. ms.
   + backward. apply IHHp2. ms.
 - apply BoxR. repeat box_tac. backward. apply IHHp. ms.
 Qed.
 
-Lemma ImpLAnd_rev Γ φ1 φ2 φ3 ψ: (Γ•(φ1 ∧ φ2 → φ3)) ⊢ ψ ->  (Γ•(φ1 → φ2 → φ3)) ⊢ ψ .
+Lemma ImpLAnd_rev {K : Kind} Γ φ1 φ2 φ3 ψ: (Γ•(φ1 ∧ φ2 → φ3)) ⊢ ψ ->  (Γ•(φ1 → φ2 → φ3)) ⊢ ψ .
 Proof.
 intro Hp.
 remember (Γ •((φ1 ∧ φ2) → φ3)) as Γ' eqn:HH.
 assert (Heq: Γ ≡ Γ' ∖ {[ ((φ1 ∧ φ2) → φ3) ]}) by ms.
 assert(Hin :((φ1 ∧ φ2) → φ3) ∈ Γ')by ms.
 rw Heq 1. clear Γ HH Heq.
-induction Hp; try forward.
-- auto with proof.
-- auto with proof.
+induction Hp.
+- forward; auto with proof.
+- forward; auto with proof.
 - apply AndR; auto with proof.
-- constructor 4. exch 0; do 2 backward. apply IHHp. ms.
+- forward; constructor 4. exch 0; do 2 backward. apply IHHp. ms.
 - apply OrR1. auto with proof.
 - apply OrR2. auto with proof.
-- constructor 7; backward; [apply IHHp1 | apply IHHp2]; ms.
+- forward; constructor 7; backward; [apply IHHp1 | apply IHHp2]; ms.
 - constructor 8. backward. apply IHHp. ms.
-- forward. exch 0. constructor 9. exch 0. do 2 backward. apply IHHp. ms.
+- do 2 forward. exch 0. constructor 9. exch 0. do 2 backward. apply IHHp. ms.
 - case (decide (((φ0 ∧ φ4) → φ5) = ((φ1 ∧ φ2) → φ3))); intro Heq0.
-  + inversion Heq0; subst. peapply Hp.
+  + dependent destruction Heq0; subst. peapply Hp.
   + forward. constructor 10. backward. apply IHHp. ms.
-- constructor 11; exch 0; do 2 backward; apply IHHp; ms.
-- constructor 12; backward; (apply IHHp1 || apply IHHp2); ms.
--  apply ImpBox; repeat box_tac.
+- forward; constructor 11; exch 0; do 2 backward; apply IHHp; ms.
+- forward; constructor 12; backward; (apply IHHp1 || apply IHHp2); ms.
+- forward; apply ImpBox; repeat box_tac.
   + exch 0; do 2 backward. apply IHHp1. ms.
   + backward. apply IHHp2. ms.
 - apply BoxR. repeat box_tac. backward. apply IHHp. ms.
@@ -449,23 +465,34 @@ Global Hint Resolve ImpLOr_rev : proof.
 Global Hint Resolve ImpLAnd_rev : proof.
 Global Hint Resolve ImpLBox_prev : proof.
 
-Lemma exfalso Γ φ: Γ ⊢ ⊥ -> Γ ⊢ φ.
+
+Lemma exfalso {K : Kind} Γ φ: Γ ⊢ ⊥ -> Γ ⊢ φ.
 Proof.
 intro Hp. dependent induction Hp; try tauto; auto with proof; tauto.
 Qed.
 
 Global Hint Immediate exfalso : proof.
 
-Lemma AndR_rev {Γ φ1 φ2} : Γ ⊢ φ1 ∧ φ2 -> (Γ ⊢ φ1) * (Γ ⊢ φ2).
-Proof. intro Hp. dependent induction Hp generalizing φ1 φ2 Hp; intuition; auto with proof. Qed.
+Lemma AndR_rev {K : Kind} {Γ φ1 φ2} : Γ ⊢ φ1 ∧ φ2 -> (Γ ⊢ φ1) * (Γ ⊢ φ2).
+Proof.
+  intro Hp. dependent induction Hp generalizing φ1 φ2 Hp;
+  try specialize (IHHp _ _ eq_refl);
+  try specialize (IHHp1 _ _ eq_refl);
+  try specialize (IHHp2 _ _ eq_refl);
+  intuition; 
+  auto with proof.
+Qed.
 
 
 (** A general inversion rule for disjunction is not admissible. However, inversion holds if one of the formulas is ⊥. *)
 
-Lemma OrR1Bot_rev Γ φ :  Γ ⊢ φ ∨ ⊥ -> Γ ⊢ φ.
-Proof. intro Hd. dependent induction Hd; auto with proof. Qed.
-Lemma OrR2Bot_rev Γ φ :  Γ ⊢ ⊥ ∨ φ -> Γ ⊢ φ.
-Proof. intro Hd. dependent induction Hd; auto with proof. Qed.
+Lemma OrR1Bot_rev {K : Kind} Γ φ :  Γ ⊢ φ ∨ ⊥ -> Γ ⊢ φ.
+Proof. intro Hd.
+ dependent induction Hd generalizing φ; auto using exfalso with proof. Qed.
+ 
+Lemma OrR2Bot_rev {K : Kind} Γ φ :  Γ ⊢ ⊥ ∨ φ -> Γ ⊢ φ.
+Proof. intro Hd. dependent induction Hd; auto using exfalso with proof. Qed.
+
 
 (** We prove Lemma 4.1 of (Dyckhoff & Negri 2000). This lemma shows that a
     weaker version of the ImpL rule of Gentzen's original calculus LJ is still
@@ -473,7 +500,7 @@ Proof. intro Hd. dependent induction Hd; auto with proof. Qed.
     proved above.
   *)
 
-Lemma weak_ImpL Γ φ ψ θ :Γ ⊢ φ -> Γ•ψ ⊢ θ -> Γ•(φ → ψ) ⊢ θ.
+Lemma weak_ImpL {K : Kind} Γ φ ψ θ :Γ ⊢ φ -> Γ•ψ ⊢ θ -> Γ•(φ → ψ) ⊢ θ.
 Proof with (auto with proof).
 intro Hp. revert ψ θ. induction Hp; intros ψ0 θ0 Hp'.
 - apply ImpLVar, Hp'.
@@ -505,7 +532,7 @@ Global Hint Resolve weak_ImpL : proof.
  G4ip. *)
 
 (** An auxiliary definition of **height** of a proof, measured along the leftmost branch. *)
-Fixpoint height {Γ φ} (Hp : Γ ⊢ φ) := match Hp with
+Fixpoint height {K : Kind} {Γ φ} (Hp : Γ ⊢ φ) := match Hp with
 | Atom _ _ => 1
 | ExFalso _ _ => 1
 | AndR Γ φ ψ H1 H2 => 1 + height H1 + height H2
@@ -522,12 +549,12 @@ Fixpoint height {Γ φ} (Hp : Γ ⊢ φ) := match Hp with
 | BoxR Γ φ H => 1 + height H
 end.
 
-Lemma height_0 {Γ φ} (Hp : Γ ⊢ φ) : height Hp <> 0.
+Lemma height_0 {K : Kind} {Γ φ} (Hp : Γ ⊢ φ) : height Hp <> 0.
 Proof. destruct Hp; simpl; lia. Qed.
 
 (** Lemma 4.2 in (Dyckhoff & Negri 2000), showing that a "duplication" in the context of the implication-case of the implication-left rule is admissible. *)
 
-Lemma ImpLImp_dup Γ φ1 φ2 φ3 θ:
+Lemma ImpLImp_dup {K : Kind} Γ φ1 φ2 φ3 θ:
   Γ•((φ1 → φ2) → φ3) ⊢ θ ->
     Γ•φ1 •(φ2 → φ3) •(φ2 → φ3) ⊢ θ.
 Proof.
@@ -560,7 +587,7 @@ destruct Hp; simpl in Hleh.
 - forward. apply ImpLAnd. backward. apply IHh with Hp. lia. ms.
 - forward. apply ImpLOr. exch 0. do 2 backward. apply IHh with Hp. lia. ms.
 - case (decide (((φ0 → φ4) → φ5) = ((φ1 → φ2) → φ3))); intro Heq.
-  + inversion Heq; subst.
+  + dependent destruction Heq; subst.
     apply weak_ImpL.
     * exch 0. apply ImpR_rev. peapply Hp1.
     * do 2 (exch 0; apply weakening). peapply Hp2.
@@ -592,7 +619,7 @@ remember (height Hp) as h.
 assert(Hleh : height Hp ≤ h) by lia. clear Heqh.
 revert Γ0 θ Hp Hleh Hin. induction h as [|h]; intros Γ θ Hp Hleh Hin;
 [pose (height_0 Hp); lia|].
-destruct Hp; simpl in Hleh.
+dependent destruction Hp; simpl in Hleh.
 - forward. auto with proof.
 - forward. auto with proof.
 - apply AndR.
@@ -613,7 +640,7 @@ destruct Hp; simpl in Hleh.
   + backward. apply IHh with Hp1. lia. ms.
   + backward. apply IHh with Hp2. lia. ms.
 - case (decide ((□ φ0 → φ3) = □ φ1 → φ2)); intro Heq.
-  + inversion Heq; subst.
+  + dependent destruction Heq; subst.
       exch 0. apply weakening. exch 0. apply weakening. peapply Hp2.
   + forward. apply ImpBox; repeat box_tac.
       * exch 0. do 2 backward.
@@ -630,20 +657,20 @@ destruct Hp; simpl in Hleh.
 Qed.
 
 (* technical lemma for contraction *)
-Local Lemma p_contr Γ φ θ:
+Local Lemma p_contr {K : Kind} Γ φ θ:
   (Γ•φ•φ) ∖ {[φ]} ⊢ θ ->
   ((Γ•φ) ⊢ θ).
 Proof. intros * Hd; peapply Hd. Qed.
 
-Lemma is_box_weight_open_box φ : is_box φ = true -> weight (⊙ φ) = weight φ -1.
-Proof. destruct φ; simpl; lia. Qed. 
+Lemma is_box_weight_open_box {K : Kind} φ : is_box φ = true -> weight (⊙ φ) = weight φ -1.
+Proof. dependent destruction φ; simpl; lia. Qed. 
 
-Lemma weight_open_box φ : weight (⊙ φ) ≤ weight φ.
-Proof. destruct φ; simpl; lia. Qed. 
+Lemma weight_open_box {K : Kind} φ : weight (⊙ φ) ≤ weight φ.
+Proof. dependent destruction φ; simpl; lia. Qed. 
 
 
 (** Admissibility of contraction in G4ip. *)
-Lemma contraction Γ ψ θ : Γ•ψ•ψ ⊢ θ -> Γ•ψ ⊢ θ.
+Lemma contraction {K : Kind} Γ ψ θ : Γ • ψ • ψ ⊢ θ -> Γ • ψ ⊢ θ.
 Proof.
 remember (Γ•ψ•ψ) as Γ0 eqn:Heq0.
 assert(HeqΓ : (Γ•ψ) ≡ Γ0 ∖ {[ψ]}) by ms.
@@ -778,7 +805,8 @@ Qed.
 
 Global Hint Resolve contraction : proof.
 
-Theorem generalised_contraction (Γ Γ' : env) φ: Γ' ⊎ Γ' ⊎ Γ ⊢ φ -> Γ' ⊎ Γ ⊢ φ.
+Theorem generalised_contraction {K : Kind} (Γ Γ' : env) φ:
+  Γ' ⊎ Γ' ⊎ Γ ⊢ φ -> Γ' ⊎ Γ ⊢ φ.
 Proof.
 revert Γ.
 induction Γ' as [| x Γ' IHΓ'] using gmultiset_rec; intros Γ Hp.
@@ -791,14 +819,14 @@ Qed.
 (** We show that the general implication left rule of LJ is admissible in G4ip.
   This is Proposition 5.2 in (Dyckhoff Negri 2000). *)
 
-Lemma ImpL Γ φ ψ θ: Γ•(φ → ψ) ⊢ φ -> Γ•ψ  ⊢ θ -> Γ•(φ → ψ) ⊢ θ.
+Lemma ImpL {K : Kind} Γ φ ψ θ: Γ•(φ → ψ) ⊢ φ -> Γ•ψ  ⊢ θ -> Γ•(φ → ψ) ⊢ θ.
 Proof. intros H1 H2. apply contraction, weak_ImpL; auto with proof. Qed.
 
 
 (* Lemma 5.3 (Dyckhoff Negri 2000) shows that an implication on the left may be
    weakened. *)
 
-Lemma imp_cut φ Γ ψ θ: Γ•(φ → ψ) ⊢ θ -> Γ•ψ ⊢ θ.
+Lemma imp_cut {K : Kind} φ Γ ψ θ: Γ•(φ → ψ) ⊢ θ -> Γ•ψ ⊢ θ.
 Proof.
 intro Hp.
 remember (Γ•(φ → ψ)) as Γ0 eqn:HH.
@@ -814,37 +842,37 @@ induction Hp.
 - forward. auto with proof.
 - forward. auto with proof.
 -apply AndR; intuition.
-- forward; apply AndL. exch 0. do 2 backward. apply IHHp. ms.
+- forward; apply AndL. exch 0. do 2 backward. apply IHHp; trivial. ms.
 - apply OrR1; intuition.
 - apply OrR2; intuition.
 - forward. apply OrL; backward; [apply IHHp1 | apply IHHp2]; ms.
-- apply ImpR. backward. apply IHHp. ms.
+- apply ImpR. backward. apply IHHp; trivial. ms.
 - case (decide ((p → φ0) = (φ → ψ))); intro Heq0.
-  + inversion Heq0; subst. peapply Hp.
+  + dependent destruction Heq0; subst. peapply Hp.
   + do 2 forward. exch 0. apply ImpLVar. exch 0. do 2 backward. apply IHHp; ms.
 - case (decide ((φ1 ∧ φ2 → φ3) = (φ → ψ))); intro Heq0.
-  + inversion Heq0; subst.
+  + dependent destruction Heq0; subst.
     assert(Heq1 : ((Γ•(φ1 ∧ φ2 → ψ)) ∖ {[φ1 ∧ φ2 → ψ]}) ≡ Γ) by ms;
     rw Heq1 1; clear Heq1. simpl in Hle.
     peapply (IHw (Γ•(φ2 → ψ)) φ2 ψ ψ0); [lia|ms|].
     peapply (IHw (Γ•(φ1 → φ2 → ψ)) φ1 (φ2 → ψ) ψ0); [lia|ms|trivial].
-  + forward. apply ImpLAnd. backward. apply IHHp. ms.
+  + forward. apply ImpLAnd. backward. apply IHHp; trivial. ms.
 - case (decide ((φ1 ∨ φ2 → φ3) = (φ → ψ))); intro Heq0.
-  + inversion Heq0. subst. clear Heq0.
+  + dependent destruction Heq0.
     apply contraction. simpl in Hle.
     peapply (IHw (Γ•ψ•(φ1 → ψ)) φ1 ψ); [lia|ms|].
     exch 0.
     peapply (IHw (Γ•(φ1 → ψ)•(φ2 → ψ)) φ2 ψ); trivial; [lia|ms].
   + forward. apply ImpLOr; exch 0; do 2 backward; apply IHHp; ms.
 - case (decide (((φ1 → φ2) → φ3) = (φ → ψ))); intro Heq0.
-  + inversion Heq0. subst. clear Heq0. peapply Hp2.
+  + dependent destruction Heq0. peapply Hp2.
   + forward. apply ImpLImp; backward; (apply IHHp1 || apply IHHp2); ms.
 - case (decide((□φ1 → φ2) = (φ → ψ))).
-  + intro Heq. inversion Heq. subst. clear Heq. peapply Hp2.
+  + intro Heq. dependent destruction Heq. peapply Hp2.
   + intro Hneq. forward. apply ImpBox; repeat box_tac.
-      * exch 0. do 2 backward. apply open_box_L. apply IHHp1. ms.
-      * backward. apply IHHp2. ms.
-- apply BoxR.  repeat box_tac. backward. apply open_box_L, IHHp.
+      * exch 0. do 2 backward. apply open_box_L. apply IHHp1; trivial. ms.
+      * backward. apply IHHp2; trivial. ms.
+- apply BoxR.  repeat box_tac. backward. apply open_box_L, IHHp; trivial.
   apply env_in_add. right. auto with proof.
 Qed.
 
@@ -857,7 +885,7 @@ induction Δ as [|ψ Δ IH] using gmultiset_rec.
 - right. ms.
 - case_eq(is_box ψ); intro Hbox.
   + left. exists (⊙ψ).
-      destruct ψ; try discriminate Hbox. ms.
+    dependent destruction ψ; try discriminate Hbox. ms.
   + destruct IH as [[φ Hφ]| Heq].
      * left. exists φ. ms.
      * right. symmetry. etransitivity.
@@ -866,13 +894,13 @@ induction Δ as [|ψ Δ IH] using gmultiset_rec.
         -- rewrite map_app, list_to_set_disj_app. rewrite <- Heq. apply env_equiv_eq.
             f_equal.
             unfold elements. apply is_not_box_open_box in Hbox.  rewrite <- Hbox at 2.
-            transitivity (list_to_set_disj (map open_box (id [ψ])) : env).
+            transitivity (list_to_set_disj (map open_box (id [ψ])) : @env Modal).
             ++ apply list_to_set_disj_perm, Permutation_map.
                     apply Permutation_refl', gmultiset_elements_singleton.
             ++ simpl. ms.
 Qed.
 
-Lemma OrR_idemp Γ ψ : Γ ⊢ ψ ∨ ψ -> Γ ⊢ ψ.
+Lemma OrR_idemp {K : Kind} Γ ψ : Γ ⊢ ψ ∨ ψ -> Γ ⊢ ψ.
 Proof. intro Hp. dependent induction Hp; auto with proof. Qed.
 
 
@@ -888,14 +916,14 @@ Qed.
   - [box_bot_not_tautology]: A boxed ⊥ cannot be a tautology.
 *)
 
-Lemma bot_not_tautology : (∅ ⊢ ⊥) -> False.
+Lemma bot_not_tautology {K : Kind} : (∅ ⊢ ⊥) -> False.
 Proof.
 intro Hf. dependent destruction Hf; simpl in *;
 match goal with x : _ ⊎ {[+?φ+]} = _ |- _ =>
 exfalso; eapply (gmultiset_elem_of_empty φ); setoid_rewrite <- x; ms end. 
 Qed.
 
-Lemma var_not_tautology v: (∅ ⊢ Var v) -> False.
+Lemma var_not_tautology {K : Kind} v: (∅ ⊢ Var v) -> False.
 Proof.
 intro Hp.
 remember ∅ as Γ.
@@ -945,7 +973,7 @@ try match goal with | Heq : (_ • ?f%stdpp) = _ |- _ => symmetry in Heq;
 Qed.
 
 (* A tautology is either equal to ⊤ or has a weight of at least 3. *)
-Lemma weight_tautology φ: (∅ ⊢ φ) -> {φ = ⊤} + {3 ≤ weight φ}.
+Lemma weight_tautology {K : Kind} φ: (∅ ⊢ φ) -> {φ = ⊤} + {3 ≤ weight φ}.
 Proof.
 intro Hp.
 destruct φ.
@@ -954,7 +982,7 @@ destruct φ.
 - right. simpl. pose(weight_pos φ1). pose(weight_pos φ2). lia.
 - right. simpl. pose(weight_pos φ1). pose(weight_pos φ2). lia.
 - right. simpl. pose(weight_pos φ1). pose(weight_pos φ2). lia.
-- destruct φ.
+- dependent destruction φ.
   + contradict Hp. apply  box_var_not_tautology.
   + contradict Hp. apply box_bot_not_tautology.
   + right. simpl. pose(weight_pos φ1). pose(weight_pos φ2). lia.
